updated more on dafny work

flightBackend.dfy
@@ -1,3 +1,6 @@
+
+datatype preferences = time | cost | flyerPoints
+
 class Date {
 	var day: int;
 	var month: int;
@@ -8,50 +11,63 @@ class Time {
 	var hour: int;
 }
 
-function method correctTime(x: Time): bool
-	reads x;
-	{
-		x != null && x.minute >= 0 && x.minute <= 60 && x.hour >= 0 && x.hour <= 60  
-	}
-
-function method correctDate(x:Date) : bool
-	reads x;
-	{
-		x != null && x.day >= 0 && x.month > 0 && x.month <= 12 
-		//since the upper bound is varied for days (28, 29, 30, 31), we can't explicitly denote that
-	}
-
 class Query {
 	var date: Date;
 	var time: Time;
 	var Start: string;
 	var Dest: string;
-	var pref1: string;
-	var pref2: string;
-	var pref3: string;
+	var pref1: preferences;
+	var pref2: preferences;
+	var pref3: preferences;
 	var numFlight: int;
-
-	constructor init () 
-		ensures correctDate(date);
-		ensures correctTime(time);
 }
 
+predicate correctPref(c:preferences)
+	ensures c in {time, cost, flyerPoints} ; 
 
-/*
-function method correctQuery (x: Query) : bool
-
+predicate correctTime(x: Time)
 	reads x;
+		ensures x != null;
+		ensures x.minute >= 0;
+		ensures x.minute < 60;
+		ensures x.hour >= 0;
+		ensures x.hour < 24;
 
-	{	
-		x != null
-	}
-*/
+predicate correctDate(x:Date)
+	reads x;
+		ensures x != null 
+		ensures x.day >= 0
+		ensures x.month > 0 
+		ensures x.month <= 12 
+		//since the upper bound is varied for days (28, 29, 30, 31), 
+		//we can't explicitly denote that, unless you want it to be <= 31...
 
-
+predicate correctQuery (x: Query)
+	reads x;
+		requires x != null;
+		requires x.time != null;
+		requires x.date != null;
+		ensures correctTime(x.time);
+		ensures correctDate(x.date);
+		ensures correctPref(x.pref1) && correctPref(x.pref2) && correctPref(x.pref3)
+		//need to ensure start and dest are in the graph class...
+		ensures x.numFlight > 0;
+		//now thinking about it...I don't think we need to have correctTime
+		//and correctDate... since the user can input invalid numbers, thus we cannot ensure this...
+		//second thoughts...we're not parsing the data here... so we need to have correct datas ...
+		//might need to ensure everything else is not null or valid
 
 method getFlightSolutions(query: Query, graph: Graph) returns (flightList: array<Trip>)
+	requires query != null;
+	requires query.date != null;
+	requires query.time != null;
+	//above keeps dafny quiet, because we're assuming that we've already parsed the required data
+	requires correctQuery(query);
+	//need to do something about the graph
 
 method searchFlights(query: Query, graph: Graph) returns (solutions: array<Trip>)
+
+
 
 method sortFlights(flightList: array<Trip>, query: Query)
 	
